# baseURI: http://www.assero.co.uk/ISO11179Identification
# imports: http://purl.org/dc/elements/1.1/
# imports: http://purl.org/dc/terms/
# imports: http://www.assero.co.uk/ISO11179Basic
# imports: http://www.assero.co.uk/ISO11179Types
# imports: http://www.w3.org/2004/02/skos/core

@prefix : <http://www.assero.co.uk/ISO11179Identification#> .
@prefix ISO11179Basic: <http://www.assero.co.uk/ISO11179Basic#> .
@prefix ISO11179Types: <http://www.assero.co.uk/ISO11179Types#> .
@prefix owl: <http://www.w3.org/2002/07/owl#> .
@prefix rdf: <http://www.w3.org/1999/02/22-rdf-syntax-ns#> .
@prefix rdfs: <http://www.w3.org/2000/01/rdf-schema#> .
@prefix skos: <http://www.w3.org/2004/02/skos/core#> .
@prefix xsd: <http://www.w3.org/2001/XMLSchema#> .

<http://www.assero.co.uk/ISO11179Identification>
  rdf:type owl:Ontology ;
  owl:imports <http://purl.org/dc/elements/1.1/> ;
  owl:imports <http://purl.org/dc/terms/> ;
  owl:imports <http://www.assero.co.uk/ISO11179Basic> ;
  owl:imports <http://www.assero.co.uk/ISO11179Types> ;
  owl:imports <http://www.w3.org/2004/02/skos/core> ;
  owl:versionInfo "Created with TopBraid Composer"^^xsd:string ;
.
:Namespace
  rdf:type owl:Class ;
  rdfs:label "Namespace"^^xsd:string ;
  rdfs:subClassOf owl:Thing ;
.
:ScopedIdentifier
  rdf:type owl:Class ;
  rdfs:label "Scoped identifier"^^xsd:string ;
  rdfs:subClassOf owl:Thing ;
  skos:definition "An identifier within a particular scope"^^xsd:string ;
.
:containedIdentifierRelationship
  rdf:type owl:ObjectProperty ;
  rdfs:domain :Namespace ;
  rdfs:label "Contained Identifier Relationship"^^xsd:string ;
  rdfs:range :ScopedIdentifier ;
  owl:inverseOf :scopeRelationship ;
.
:identifiedItemRelationship
  rdf:type owl:ObjectProperty ;
  rdfs:domain :ScopedIdentifier ;
  rdfs:label "Identified Item Relationship"^^xsd:string ;
  rdfs:range ISO11179Types:IdentifiedItem ;
  skos:definition "Identifies the Identified_Item defined by the Scoped_Identifier"^^xsd:string ;
.
:identifier
  rdf:type owl:DatatypeProperty ;
  rdfs:domain :ScopedIdentifier ;
  rdfs:label "identifier"^^xsd:string ;
  rdfs:range xsd:string ;
  skos:definition "String used to unambiguously denote an IdentifiedItem within the scope of a specified Namespace."^^xsd:string ;
.
:identifierRelationship
  rdf:type owl:ObjectProperty ;
  rdfs:domain ISO11179Types:IdentifiedItem ;
  rdfs:label "Identifer Relationship"^^xsd:string ;
  rdfs:range :ScopedIdentifier ;
  skos:definition "Identifies the set of Scope_Identifiers for the Identified_Item that defines an identifier within a specific namespace"^^xsd:string ;
.
:namingAuthority
  rdf:type owl:DatatypeProperty ;
  rdfs:domain :Namespace ;
  rdfs:label "Naming Authority"^^xsd:string ;
  rdfs:range ISO11179Basic:Organization ;
  skos:definition "Organization that has the authroity for naming in the namespace"^^xsd:string ;
.
:scopeRelationship
  rdf:type owl:ObjectProperty ;
  rdfs:domain :ScopedIdentifier ;
  rdfs:label "Scope Relationship"^^xsd:string ;
  rdfs:range :Namespace ;
.
:version
  rdf:type owl:DatatypeProperty ;
  rdfs:domain :ScopedIdentifier ;
  rdfs:label "version"^^xsd:string ;
  rdfs:range xsd:string ;
  skos:definition "Unique version identifier of the ScopedIdentifier which identifies an IdentifiedItem"^^xsd:string ;
.
